Refined.v
@@ -29,9 +29,7 @@ Record PS := makePS {
   psBufLen : N;
 
   psOffset : N;
-  psLength : N;
-
-  psError  : bool
+  psLength : N
 }.
 
   (* psBufInHeap : psBufLen = 0 \/ Ensembles.In _ (fst heap) (psBuffer, psBufLen); *)
@@ -39,91 +37,376 @@ Record PS := makePS {
   (* psBegInBlock : psBufLen = 0 \/ within psBuffer psBufLen psOffset; *)
   (* psEndInBlock : psBufLen = 0 \/ within psBuffer psBufLen (psOffset + psLength) *)
 
-Definition ByteString_list_AbsR (or : Rep ByteStringSpec) (nr : PS) :=
-  forall i x (H : (N.to_nat i <? length or)%nat),
-    x = nth_safe (N.to_nat i) or H
-      <-> (x <- peek (psHeap nr) (psOffset nr); ret (snd x)) ↝ Some x.
+Theorem Nle_zero : forall n : N, 0 <= n.
+Proof.
+  destruct n.
+    reflexivity.
+  destruct p; discriminate.
+Qed.
 
-(*
+Theorem Nlt_plus_1 : forall n : N, 0 < n + 1.
+Proof.
+  destruct n.
+    reflexivity.
+  constructor.
+Qed.
+
+Theorem Nsucc_nat : forall n, N.pos (Pos.of_succ_nat n) = N.succ (N.of_nat n).
+Proof.
+  induction n.
+    reflexivity.
+  constructor.
+Qed.
+
+Theorem Nsub_add_succ : forall n m,
+  n - 1 + N.succ (N.of_nat m) = n + N.of_nat m.
+Proof.
+  destruct n; intros.
+    admit.
+  admit.
+Admitted.
+
+Theorem Nplus_1_mismatch : forall n m, n > 0 -> n + m = n - 1 -> False.
+Proof.
+  destruct n; intros.
+    discriminate.
+Admitted.
+
+Theorem Nlt_false : forall n, (0 <? n) = false -> n = 0.
+Proof.
+  destruct n; intros.
+    reflexivity.
+  discriminate.
+Qed.
+
+Theorem within_extended : forall addr len i,
+  within (addr - 1) (len + 1) (N.succ i) -> within addr len i.
+Proof.
+  unfold within; intros.
+  destruct H.
+  split.
+    admit.
+  admit.
+Admitted.
+
+Definition ByteString_list_AbsR (or : Rep ByteStringSpec) (nr : PS) :=
+  length or = N.to_nat (psLength nr) /\
+  forall i x,
+    (i <? length or)%nat
+      -> within (psOffset nr) (psLength nr) (N.of_nat i)
+      -> x = nth i or x <->
+         (x <- peek (psHeap nr) (psOffset nr + N.of_nat i);
+          ret (snd x)) ↝ Some x.
+
+Definition buffer_cons (r : PS) (d : Word8) : Comp PS :=
+  ps <- If 0 <? psOffset r
+        Then ret {| psHeap   := psHeap r
+                  ; psBuffer := psBuffer r
+                  ; psBufLen := psBufLen r
+                  ; psOffset := psOffset r - 1
+                  ; psLength := psLength r + 1 |}
+        Else (
+          If psLength r <? psBufLen r
+          Then res <- memcpy (psHeap r) (psBuffer r)
+                             (psBuffer r + 1) (psLength r);
+               ret {| psHeap   := fst res
+                    ; psBuffer := psBuffer r
+                    ; psBufLen := psBufLen r
+                    ; psOffset := 0
+                    ; psLength := psLength r + 1 |}
+          Else (
+            res <- realloc (psHeap r) (psBuffer r)
+                           (exist _ (psLength r + 1)
+                                    (Nlt_plus_1 _));
+            ret {| psHeap   := fst res
+                 ; psBuffer := snd res
+                 ; psBufLen := psLength r + 1
+                 ; psOffset := 0
+                 ; psLength := psLength r + 1 |}));
+  res <- poke (psHeap ps) (psOffset ps) d;
+  ret {| psHeap   := fst res
+       ; psBuffer := psBuffer ps
+       ; psBufLen := psBufLen ps
+       ; psOffset := psOffset ps
+       ; psLength := psLength ps |}.
+
+Ltac reduction :=
+  repeat match goal with
+    | [ H : Some _ = Some _ |- _ ] => inv H
+    | [ H : (_, _) = (_, _) |- _ ] => inv H
+    (* | [ _ : is_true (Nat.ltb 0 _) |- _ ] => *)
+    (*   rewrite N.add_0_r in *; *)
+    (*   try (apply Union_intror; constructor) *)
+    | [ H : forall x : _, Some ?X = Some x -> _ |- _ ] =>
+      specialize (H X eq_refl);
+      simplify_ensembles; subst; simpl in *
+    | [ |- context [N.pos (Pos.of_succ_nat _)] ] =>
+      rewrite Nsucc_nat
+    | [ H : context [N.pos (Pos.of_succ_nat _)] |- _ ] =>
+      rewrite Nsucc_nat in H
+    | [ |- context [N.succ (N.of_nat _)] ] =>
+      rewrite Nsub_add_succ
+    | [ H : context [N.succ (N.of_nat _)] |- _ ] =>
+      rewrite Nsub_add_succ in H
+    | [ H1 : is_true (Nat.ltb (S ?I) (S _)),
+        _  : _ = nth ?I _ ?X,
+        H2 : forall i x, is_true (Nat.ltb i _) -> _ |- _ ] =>
+      specialize (H2 I X H1); clear H1
+    | [ H1 : is_true (Nat.ltb (S ?I) (S _)),
+        _  : In _ _ (_, ?X),
+        H2 : forall i x, is_true (Nat.ltb i _) -> _ |- _ ] =>
+      specialize (H2 I X H1); clear H1
+    | [ H1 : _ = nth _ _ _,
+        H2 : _ = nth _ _ _ <-> _ |- _ ] =>
+      apply H2 in H1; clear H2;
+      simplify_ensembles; subst; simpl in *
+    | [ H : _ = nth _ _ _ <-> _ |- _ = nth _ _ _ ] =>
+      apply H; clear H;
+      autorewrite with monad laws;
+      simplify_ensembles; simpl; intros
+    | [ |- ~ _ ] => unfold not; intros
+    end.
+
+Theorem buffer_cons_sound
+        (r_o : list Word8) (r_n : PS) (x : Word8)
+        (AbsR : ByteString_list_AbsR r_o r_n) :
+  forall r_n', buffer_cons r_n x ↝ r_n' ->
+    ByteString_list_AbsR (x :: r_o) r_n'.
+Proof.
+  unfold buffer_cons, ByteString_list_AbsR,
+         peek, poke, memcpy.
+  simpl; intros.
+  destruct AbsR.
+  rewrite H0 in *; clear H0.
+
+  split.
+    destruct (0 <? psOffset r_n) eqn:Heqe;
+    destruct (psLength r_n <? psBufLen r_n);
+    clear -H; simpl in H;
+    simplify_ensembles; subst; simpl;
+    rewrite <- N2Nat.inj_succ, N.add_1_r; reflexivity.
+
+  split; intros.
+    autorewrite with monad laws.
+    apply PickComputes; intros ? H4; inv H4.
+    destruct (psLength r_n <? psBufLen r_n);
+    (destruct (0 <? psOffset r_n) eqn:Heqe;
+     [|apply Nlt_false in Heqe]);
+    simplify_ensembles; subst; simpl in *; inv H4;
+    (destruct i; subst;
+     [apply Union_intror|apply Union_introl]);
+    rewrite ?N.add_0_r, ?Heqe in *;
+    try constructor;
+    unfold peek in *;
+    simplify_ensembles; subst; simpl in *;
+    reduction.
+    simpl in H;
+    + inv H3.
+      destruct i; subst; [apply Union_intror|apply Union_introl].
+        constructor.
+      specialize (H1 i x1 H0).
+      apply H1 in H2; clear H1 H0.
+      unfold peek in H2.
+      simplify_ensembles.
+        simpl in H0.
+        admit.
+      unfold not; intros.
+      inv H2.
+      admit.
+    + inv H3.
+      destruct i; subst; [apply Union_intror|apply Union_introl].
+        rewrite N.add_0_r.
+        constructor.
+      specialize (H1 i x1 H0).
+      apply H1 in H2; clear H1 H0.
+      unfold peek in H2.
+      simplify_ensembles.
+        simpl in H0.
+        admit.
+      unfold not; intros.
+      inv H2.
+      admit.
+    + inv H3.
+      destruct i; subst; [apply Union_intror|apply Union_introl].
+        constructor.
+      specialize (H1 i x1 H0).
+      apply H1 in H2; clear H1 H0.
+      unfold peek in H2.
+      simplify_ensembles.
+        simpl in H0.
+        admit.
+      unfold not; intros.
+      inv H2.
+    + 
+        rewrite N.ltb_lt in Heqe.
+        apply N.lt_gt.
+    inv H3.
+
+  destruct i; [clear H1 H0|].
+    destruct (0 <? psOffset r_n) eqn:Heqe;
+    destruct (psLength r_n <? psBufLen r_n);
+    simpl in H;
+    simplify_ensembles; subst; simpl in *.
+
+  (split; intros; [autorewrite with monad laws|]);
+  simplify_ensembles; intro; subst; simpl in *.
+      split.
+
+      split; intros;
+      unfold poke in H0.
+        autorewrite with monad laws.
+        destruct (0 <? psOffset r_n) eqn:Heqe;
+        destruct (psLength r_n <? psBufLen r_n);
+        simpl in H0;
+        simplify_ensembles;
+        subst; simpl in *; intros;
+        repeat match goal with
+          | [ H : Some _ = Some _ |- _ ] => inv H
+          | [ H : (_, _) = (_, _) |- _ ] => inv H
+          end.
+        admit.
+        admit.
+        admit.
+        admit.
+
+      unfold peek in H3.
+      simplify_ensembles.
+      repeat match goal with
+        | [ H : Some _ = Some _ |- _ ] => inv H
+        | [ H : (_, _) = (_, _) |- _ ] => inv H
+        end.
+      simpl in *.
+      specialize (H3 x H4).
+      repeat match goal with
+        | [ H : Some _ = Some _ |- _ ] => inv H
+        | [ H : (_, _) = (_, _) |- _ ] => inv H
+        end.
+      destruct (0 <? psOffset r_n) eqn:Heqe;
+      destruct (psLength r_n <? psBufLen r_n);
+      simpl in H0;
+      simplify_ensembles;
+      subst; simpl in *; intros.
+
+      destruct i; split; intros; subst;
+      autorewrite with monad laws;
+      simplify_ensembles;
+      intros; simpl in *;
+      repeat match goal with
+        | [ H : Some _ = Some _ |- _ ] => inv H
+        | [ H : (_, _) = (_, _) |- _ ] => inv H
+        | [ _ : is_true (Nat.ltb 0 _) |- _ ] =>
+          rewrite N.add_0_r in *;
+          try (apply Union_intror; constructor)
+        | [ H : forall x : _, Some ?X = Some x -> _ |- _ ] =>
+          specialize (H X eq_refl);
+          simplify_ensembles; subst; simpl in *
+        | [ |- context [N.pos (Pos.of_succ_nat _)] ] =>
+          rewrite Nsucc_nat
+        | [ H : context [N.pos (Pos.of_succ_nat _)] |- _ ] =>
+          rewrite Nsucc_nat in H
+        | [ |- context [N.succ (N.of_nat _)] ] =>
+          rewrite Nsub_add_succ
+        | [ H : context [N.succ (N.of_nat _)] |- _ ] =>
+          rewrite Nsub_add_succ in H
+        | [ H1 : is_true (Nat.ltb (S ?I) (S _)),
+            _  : _ = nth ?I _ ?X,
+            H2 : forall i x, is_true (Nat.ltb i _) -> _ |- _ ] =>
+          specialize (H2 I X H1); clear H1
+        | [ H1 : is_true (Nat.ltb (S ?I) (S _)),
+            _  : In _ _ (_, ?X),
+            H2 : forall i x, is_true (Nat.ltb i _) -> _ |- _ ] =>
+          specialize (H2 I X H1); clear H1
+        | [ H1 : _ = nth _ _ _,
+            H2 : _ = nth _ _ _ <-> _ |- _ ] =>
+          apply H2 in H1; clear H2;
+          simplify_ensembles; subst; simpl in *
+        | [ H : _ = nth _ _ _ <-> _ |- _ = nth _ _ _ ] =>
+          apply H; clear H;
+          autorewrite with monad laws;
+          simplify_ensembles; simpl; intros
+        | [ |- ~ _ ] => unfold not; intros
+        | [ |- In _ _ _ ] => apply Union_introl; split; intros
+        end.
+
+      - inv H1.
+        apply Nplus_1_mismatch in H3.
+          assumption.
+        rewrite N.ltb_lt in Heqe.
+        apply N.lt_gt.
+        assumption.
+      - assumption.
+      - symmetry in H4.
+        apply Nplus_1_mismatch in H4.
+          contradiction.
+        rewrite N.ltb_lt in Heqe.
+        apply N.lt_gt.
+        assumption.
+      - inv H1.
+        apply Nplus_1_mismatch in H3.
+          assumption.
+        rewrite N.ltb_lt in Heqe.
+        apply N.lt_gt.
+        assumption.
+      - assumption.
+      - symmetry in H4.
+        apply Nplus_1_mismatch in H4.
+          contradiction.
+        rewrite N.ltb_lt in Heqe.
+        apply N.lt_gt.
+        assumption.
+      - clear H1 H0 Heqe.
+        admit.
+      - inv H2.
+        admit.
+      - admit.
+      - inv H1.
+        admit.
+      - contradiction H4.
+        unfold Ensembles.In; simpl.
+        admit.
+      - admit.
+      - admit.
+      - admit.
+      - admit.
+      - admit.
+    }
+    finish honing.
+  }
+Admitted.
+
 Lemma ByteStringImpl (heap : Rep HeapSpec) : FullySharpened ByteStringSpec.
 Proof.
   start sharpening ADT.
   unfold ByteStringSpec; simpl.
-  hone representation using ByteString_list_AbsR;
-  try simplify with monad laws; simpl;
-  unfold ByteString_list_AbsR in *.
+  hone representation using ByteString_list_AbsR.
   {
+    simplify with monad laws.
     refine pick val
       {| psHeap   := heap
        ; psBuffer := 0
        ; psBufLen := 0
        ; psOffset := 0
-       ; psLength := 0
-       ; psError  := false |}; simpl.
+       ; psLength := 0 |}.
       finish honing.
-    split; intros; inv H0.
+    split; intros.
+      reflexivity.
+    split; intros; discriminate.
   }
   {
+    simplify with monad laws.
     etransitivity.
-      apply (refine_skip2 (dummy:=realloc (psHeap r_n) (psBuffer r_n)
-                                          (psLength r_n + 1))).
+      eapply (refine_skip2 (dummy:=buffer_cons r_n d)).
     etransitivity.
       apply refine_under_bind; intros.
-      refine pick val
-        (if psError r_n
-         then r_n
-         else if 0 <? psOffset r_n
-              then {| psHeap   := heap
-                      ; psBuffer := psBuffer r_n
-                      ; psBufLen := psBufLen r_n
-                      ; psOffset := psOffset r_n - 1
-                      ; psLength := psLength r_n + 1
-                      ; psError  := false |}
-              else if psBuffer r_n + psOffset r_n + psLength r_n + 1 <=?
-                      psBuffer r_n + psBufLen r_n
-                   then {| psHeap   := heap
-                         ; psBuffer := psBuffer r_n
-                         ; psBufLen := psBufLen r_n
-                         ; psOffset := psOffset r_n
-                         ; psLength := psLength r_n + 1
-                         ; psError  := false |}
-                   else match snd a with
-                        | Some addr =>
-                          {| psHeap   := fst a
-                           ; psBuffer := addr
-                           ; psBufLen := psLength r_n + 1
-                           ; psOffset := 0
-                           ; psLength := psLength r_n + 1
-                           ; psError  := false |}
-                        | None =>
-                          {| psHeap   := fst a
-                           ; psBuffer := psBuffer r_n
-                           ; psBufLen := psBufLen r_n
-                           ; psOffset := psOffset r_n
-                           ; psLength := psLength r_n
-                           ; psError  := true |}
-                        end); simpl.
+      refine pick val a.
         simplify with monad laws.
         finish honing.
-      intros.
-      specialize (H0 i x).
-      destruct (psError r_n); intros.
-        split; intros; subst.
-          eapply BindComputes.
-            unfold peek.
-            eapply BindComputes.
-              apply PickComputes; intros.
-      destruct (0 <? psOffset r_n); simpl.
-        admit.
-      destruct (psBuffer r_n + psOffset r_n + psLength r_n + 1 <=?
-                psBuffer r_n + psBufLen r_n); simpl.
-        admit.
-      destruct a, o; simpl.
-        admit.
-      admit.
-    simpl.
+      exact (buffer_cons_sound H0 H1).
+    unfold buffer_cons.
+    simplify with monad laws; simpl.
     finish honing.
   }
+  (*
   {
     refine pick val (match r_n with
                      | nil => (r_o, None)
@@ -193,12 +476,15 @@ Proof.
         reflexivity.
       reflexivity.
   }
+  *)
+  admit.
 
   finish_SharpeningADT_WithoutDelegation.
-Defined.
+  simpl.
+Fail Defined.
 
-Definition ByteStringImpl' := Eval simpl in projT1 ByteStringImpl.
+Fail Definition ByteStringImpl' := Eval simpl in projT1 ByteStringImpl.
 (* Print ByteStringImpl'. *)
-*)
 
-End ByteString.
+Fail End ByteString.
+Abort All.
